adding SepLogFold (moved from Cancel)

MirrorCharge!/src/Cancel.v
@@ -4,10 +4,13 @@
  ** - Support star and emp
  **)
 Require Import ExtLib.Data.Positive.
+Require Import ExtLib.Tactics.
 Require Import BILogic.
+Require Import MirrorCore.EnvI.
+Require Import MirrorCore.SymI.
 Require Import MirrorCore.Ext.Expr.
 Require Import MirrorCore.Ext.AppFull.
-Require Import ILogicFunc.
+Require Import ILogicFunc SepLogFold.
 
 Set Implicit Arguments.
 Set Strict Implicit.
@@ -20,7 +23,7 @@ Section cancel_state.
     {| spacial := nil |}.
 
   Definition atomic e : conjunctives :=
-    {| spacial := (e,nil) :: nil |}.
+    {| spacial := app_full e :: nil |}.
 
   Definition atomic_app e es : conjunctives :=
     {| spacial := (e, es) :: nil |}.
@@ -60,9 +63,40 @@ Section cancel_state.
     Definition inj_star a b :=
       Eval compute in apps (Inj (fref 1%positive)) (a :: b :: nil).
 
-    Definition test := app_fold_args normalizeArgs.
+    Definition test := fun x => app_fold_args normalizeArgs x nil nil.
     Eval compute in  test inj_emp.
     Eval compute in  test (inj_star inj_emp inj_emp).
     Eval compute in  test (inj_star (Var 0) (inj_star inj_emp (inj_and (Var 1) (Var 3)))).
   End demo.
+
+  Require Import ExtLib.Structures.Monads.
+  Require Import ExtLib.Data.Monads.StateMonad.
+
+  Section with_monad.
+    Local Open Scope monad_scope.
+    Import MonadNotation.
+
+    Definition conjunctives_remove (c : conjunctives) (e : expr ilfunc)
+    : option conjunctives:= None.
+
+  Definition cancel_atomic (e : expr ilfunc) : state conjunctives conjunctives :=
+    (lhs <- get ;;
+     match conjunctives_remove lhs e with
+       | None => (** it wasn't found **)
+         ret (atomic e)
+       | Some r =>
+         put r ;;
+         ret empty
+     end)%monad.
+
+  Definition cancelArgs : AppFullFoldArgs ilfunc (state conjunctives conjunctives) :=
+  {| do_var := fun v _ _ => cancel_atomic (Var v)
+   ; do_uvar := fun u _ _ => cancel_atomic (UVar u)
+   ; do_inj := fun i _ _ => cancel_atomic (Inj i)
+   ;
+
+
+  Definition cancel (rhs : expr ilfunc) : conjunctives -> (conjunctives * conjunctives).
+
+
 End cancel_state.
