MirrorCharge!/src/SepLogFold.v
@@ -1,0 +1,201 @@
+(** This file implements an interface to [expr] that
+ ** makes star, emp, and pure assertions apparent.
+ **)
+Require Import ExtLib.Data.Positive.
+Require Import ExtLib.Tactics.
+Require Import BILogic.
+Require Import MirrorCore.EnvI.
+Require Import MirrorCore.SymI.
+Require Import MirrorCore.Ext.Expr.
+Require Import MirrorCore.Ext.AppFull.
+Require Import ILogicFunc.
+
+Set Implicit Arguments.
+Set Strict Implicit.
+
+Section seplog_fold.
+  Variable ts : types.
+  Variable sym : Type.
+  Variable RSym_sym : RSym (typD ts) sym.
+
+  Variable T : Type.
+
+  Record SepLogArgs : Type :=
+  { do_atomic_app : expr sym -> list (expr sym) -> T
+  ; do_pure : expr sym -> T
+  ; do_emp : T
+  ; do_star : T -> T -> T
+  }.
+
+  Variable is_pure : expr sym -> bool.
+  Variable is_emp : sym -> bool.
+  Variable is_star : sym -> bool.
+
+  Record SepLogArgsOk (ST : typ) (sla : SepLogArgs) : Type :=
+  { R_t : expr sym -> T -> tenv typ -> tenv typ -> Prop
+  ; Hatomic_app
+    : forall e es tus tvs,
+        typeof_apps _ tus tvs e es = Some ST ->
+        R_t (apps e es) (sla.(do_atomic_app) e es) tus tvs
+  ; Hpure
+    : forall e tus tvs,
+        typeof_expr tus tvs e = Some ST ->
+        is_pure e = true ->
+        R_t e (sla.(do_pure) e) tus tvs
+  ; Hemp
+    : forall e tus tvs,
+        typeof_sym e = Some ST ->
+        is_emp e = true ->
+        R_t (Inj e) sla.(do_emp) tus tvs
+  ; Hstar
+    : forall e l r l_res r_res tus tvs,
+        typeof_sym e = Some (tyArr ST (tyArr ST ST)) ->
+        typeof_expr tus tvs l = Some ST ->
+        typeof_expr tus tvs r = Some ST ->
+        is_star e = true ->
+        R_t l l_res tus tvs ->
+        R_t r r_res tus tvs ->
+        R_t (apps (Inj e) (l :: r :: nil)) (sla.(do_star) l_res r_res) tus tvs
+  }.
+
+  Definition AppFullFoldArgs_SepLogArgs (sla : SepLogArgs) : AppFullFoldArgs sym T :=
+    match sla with
+      | {| do_atomic_app := do_atomic_app
+         ; do_pure := do_pure
+         ; do_star := do_star
+         ; do_emp := do_emp |} =>
+        {| do_var := fun v _ _ => do_atomic_app (Var v) nil
+         ; do_uvar := fun u _ _ => do_atomic_app (UVar u) nil
+         ; do_inj := fun i _ _ =>
+                       if is_emp i then
+                         do_emp
+                       else
+                         do_atomic_app (Inj i) nil
+         ; do_abs := fun t e _ _ _ => do_atomic_app (Abs t e) nil
+         ; do_app := fun f _ args tus tvs =>
+                       match f with
+                         | Inj i =>
+                           if is_star i then
+                             match args with
+                               | (_,l) :: (_,r) :: nil =>
+                                 do_star (l tus tvs) (r tus tvs)
+                               | _ => do_emp
+                             end
+                           else
+                             do_atomic_app f (map fst args)
+                         | _ =>
+                           do_atomic_app f (map fst args)
+                       end
+        |}
+    end.
+
+  Section sound.
+    Context SL sla `{slaok : SepLogArgsOk SL sla}.
+
+    Lemma atomic_ok
+    : forall (tus tvs : tenv typ) e (t : typ),
+        typeof_expr tus tvs e = Some t ->
+        t = SL ->
+        R_t slaok e (sla.(do_atomic_app) e nil) tus
+            tvs.
+    Proof.
+      destruct sla; simpl; intros; subst.
+      change e with (apps e nil) at 1.
+      eapply Hatomic_app. unfold typeof_apps.
+      simpl. rewrite H. auto.
+    Qed.
+
+    Hypothesis BILOps : BILOperators (typD ts nil SL).
+    Hypothesis is_starOk
+    : forall i,
+        is_star i = true ->
+        let starT := tyArr SL (tyArr SL SL) in
+        exists pf : typeof_sym i = Some starT,
+          sepSP = match pf in _ = u
+                        return match u with
+                                 | Some t => typD ts nil t
+                                 | None => unit
+                               end
+                  with
+                    | eq_refl => symD i
+                  end.
+
+    Definition AppFullFoldArgsOk_SepLogsOk
+    : AppFullFoldArgsOk _ (AppFullFoldArgs_SepLogArgs sla).
+    Proof.
+      refine (
+          @Build_AppFullFoldArgsOk _ _ _ _ _
+                                   (fun t e res tus tvs =>
+                                      t = SL ->
+                                      slaok.(R_t) e res tus tvs)
+                                   _ _ _ _ _).
+      { destruct sla; simpl; intros; subst.
+        change (Var v) with (apps (@Var sym v) nil) at 1.
+        eapply Hatomic_app. unfold typeof_apps.
+        simpl; rewrite H; auto. }
+      { destruct sla; simpl; intros; subst.
+        change (UVar v) with (apps (@UVar sym v) nil) at 1.
+        eapply Hatomic_app. unfold typeof_apps.
+        simpl. rewrite H. auto. }
+      { destruct sla; simpl; intros; subst.
+        change (Inj v) with (apps (@Inj sym v) nil) at 1.
+        consider (is_emp v); intros.
+        { eapply Hemp; eauto. }
+        { eapply Hatomic_app. unfold typeof_apps.
+          simpl. rewrite H. auto. } }
+      { destruct sla; simpl; intros; subst.
+        change (Abs t e) with (apps (Abs t e) nil) at 1.
+        eapply Hatomic_app. unfold typeof_apps.
+        simpl. rewrite H. auto. }
+      { intros. subst ft. subst.
+        destruct sla; simpl.
+        assert (typeof_apps RSym_sym tus tvs l (map fst rs) = Some SL).
+        { rewrite <- typeof_expr_apps. auto. }
+        destruct l; try solve [ eapply Hatomic_app; eauto ].
+        consider (is_star s); intros.
+        { generalize H3. eapply is_starOk in H3. destruct H3.
+          unfold typeof_apps in H2.
+          simpl in H2. rewrite x in H2.
+          destruct rs; simpl in *.
+          { rewrite x in H. clear - H. inv_all.
+            symmetry in H. eapply tyArr_circ_L in H. intuition. }
+          { inversion H1; clear H1; subst.
+            inversion H8; clear H8; subst.
+            { subst. simpl in *. forward; inv_all; try subst.
+              exfalso. eapply tyArr_circ_L; eauto. }
+            { subst. inversion H4; clear H4; subst.
+              { forward. subst. simpl in *.
+                inv_all; subst.
+                intuition. inv_all; subst.
+                rewrite H in *. rewrite H7 in *. rewrite x in *.
+                unfold type_of_apply in *.
+                forward. inv_all. revert H9. subst.
+                intro.
+                eapply Hstar; eauto. }
+              { intuition. simpl in *.
+                rewrite typeof_expr_apps in H.
+                unfold typeof_apps in H. simpl in H.
+                rewrite H8 in *. rewrite H7 in *. rewrite H1 in *.
+                rewrite x in *.
+                unfold type_of_apply in *.
+                forward; inv_all; subst. inv_all; subst.
+                eapply type_of_applys_circle_False in H14. intuition. } } } }
+        { eapply Hatomic_app; eauto. } }
+    Defined.
+
+    Definition seplog_fold (sla : SepLogArgs) : expr sym -> tenv typ -> tenv typ -> T :=
+      app_fold_args (AppFullFoldArgs_SepLogArgs sla).
+
+    Theorem seplog_fold_sound
+    : forall e tus tvs result,
+        seplog_fold sla e tus tvs = result ->
+        typeof_expr tus tvs e = Some SL ->
+        slaok.(R_t) e result tus tvs.
+    Proof.
+      intros.
+      eapply app_fold_args_sound in H. 2: eapply H0.
+      revert H. instantiate (1 := AppFullFoldArgsOk_SepLogsOk).
+      simpl. intuition.
+    Qed.
+  End sound.
+End seplog_fold.
